---
title: "[]{#_bzwks5sw9lxj .anchor}From the Fourier series to the Fourier transform"
---

# Introduction

- [The Fourier transform](?tab=t.lu5907fvi1t4) blog post gives the definition of the Fourier transform.

<!-- -->

- But it does not explain where it comes from.

- This blog post explains where the Fourier transform comes from.

# Summary

The post is organized as follows

- The [Fourier series](#fourier-series-1) section explains that

  - Fourier had the intuition (but no proof) for the following equality for periodic signals (see [Fourier's intuition](#fouriers-intuition))

> $f(t) = \frac{a_{0}}{2} + \sum_{n = 1}^{\infty}\left\lbrack a_{n}cos(2\pi n\xi t) + b_{n}sin(2\pi n\xi t) \right\rbrack$ (1)

- This expression can be rewritten as (see [From sine/cosine to complex exponentials](#from-sinecosine-to-complex-exponentials))

> $f(t) = \sum_{n = - \infty}^{\infty}c_{n}e^{i2\pi n\xi t}$ (2)

- Which makes

  - Complex exponentials appear.

  - Positive and negative frequencies appear.

- The corresponding Fourier series coefficients can be derived from orthogonality as (see [From Fourier series intuition to Fourier series coefficients](#from-fourier-series-intuition-to-fourier-series-coefficients))

> $c_{n} = \frac{1}{T}\int_{0}^{T}f(t)\ e^{- i2\pi n\xi t}dt$

- The [From the Fourier Series to the Fourier Transform](#from-the-fourier-series-to-the-fourier-transform) section explains that

  - The [Fourier series](#fourier-series-1) intuition can be extended to a non-periodic signal by seeing it as the limit of a periodic signal as its period $T \rightarrow \infty$.

  - This leads to (see [From the Fourier Series to the Fourier Transform](#from-the-fourier-series-to-the-fourier-transform))

> $f(t) = \int_{- \infty}^{\infty}F(\xi)e^{i2\pi\xi t}d\xi$ (3)

- Note that even though expression (3) is the limit of the Fourier series (expression (2)) as $T \rightarrow \infty$, it is **not** called the Fourier transform.

  - In fact, it is the inverse Fourier transform instead.

  - The Fourier transform is the function $F(\xi)$ of $\xi$ (i.e. the Fourier transform coefficients).

- Similarly to the Fourier series, this leads to the Fourier transform coefficients

> $F(\xi) = \int_{- \infty}^{\infty}f(t)\ e^{- i2\pi\xi t}dt$

# Fourier series

- This section explains Fourier\'s intuition that led to the Fourier series and the Fourier series coefficients.

## Fourier's intuition

- Fourier had the intuition that any periodic signal with period $T$ (or frequency $\xi = \frac{1}{T}$) can be decomposed as an infinite sum of oscillations at frequencies that are integer multiples of $\xi$.

- [He did not prove this intuition](https://proofwiki.org/wiki/Definition:Fourier_Series/Historical_Note).

- He used it as an assumption and derived the Fourier series coefficients from this assumption.

- The empirical success suggested that the assumption was correct.

- But mathematical proof came later.

  - Dirichlet provided the first rigorous proof in 1829, valid under certain conditions now called the Dirichlet conditions.

  - This proof is only valid for Fourier series / periodic signals.

  - Hence, this proof does not apply to modern Fourier analysis of non-periodic signals.

  - One must refer to the convergence proof of the inverse Fourier transform instead (see the [Signal decomposition](?tab=t.lu5907fvi1t4#heading=h.8eku66x31rxt) section of [The Fourier transform](?tab=t.lu5907fvi1t4#heading=h.bzwks5sw9lxj) blog post).

## Fourier series

- Fourier's assumption

  - For a periodic signal with period $T$ (or frequency $\xi = \frac{1}{T}$)

  - and with $n$ an integer.

> $f(t) = \frac{a_{0}}{2} + \sum_{n = 1}^{\infty}\left\lbrack a_{n}cos(2\pi n\xi t) + b_{n}sin(2\pi n\xi t) \right\rbrack$ (1)

- As explained in the [Representations of an oscillation](#_8kvw1n73y17q) section of the [Fourier transform](?tab=t.lu5907fvi1t4) blog post, complex exponentials are easier to manipulate.

- As shown in the [From sine/cosine to complex exponentials](#from-sinecosine-to-complex-exponentials) section below, expression (1) above be rewritten as

$f(t) = \sum_{n = - \infty}^{\infty}c_{n}e^{i2\pi n\xi t}$ (2)

## Fourier series coefficients

- The [From Fourier series intuition to Fourier series coefficients](#from-fourier-series-intuition-to-fourier-series-coefficients) shows that

> $c_{n} = \frac{1}{T}\int_{0}^{T}f(t)\ e^{- i2\pi n\xi t}dt$

# From the Fourier Series to the Fourier Transform

- This section explains how the Fourier transform can then be derived from the Fourier series.

<!-- -->

- In expression (2) above, the infinite sum is discrete.

  - It is the sum over the integer multiples of $\xi$.

  - All the terms in the sum are evenly spaced every $\xi$.

  - Where $\xi = \frac{1}{T}$ and $T$ is the period of the periodic signal.

- A non-periodic signal can be seen as the limit of a periodic signal as its period $T \rightarrow \infty$.

  - As $T \rightarrow \infty$,

  - $\xi = \frac{1}{T} \rightarrow 0$.

  - Hence, the spacing between the terms in the sum tends toward $0$,

  - and the sum becomes an integral.

  - This gives

> $f(t) = \int_{- \infty}^{\infty}c_{\xi}e^{i2\pi\xi t}d\xi$

- If $c_{\xi}$ is written as $F(\xi)$ instead, this gives

> $f(t) = \int_{- \infty}^{\infty}F(\xi)e^{i2\pi\xi t}d\xi$ (3)

- Which is the same as expression (2) in the [Fourier transform](?tab=t.lu5907fvi1t4) blog post.

<!-- -->

- Note that even though expression (3) is the limit of the Fourier series (expression (2)) as $T \rightarrow \infty$, it is **not** called the Fourier transform.

  - In fact, it is the inverse Fourier transform instead.

  - The Fourier transform is the function $F(\xi)$ of $\xi$ (i.e. the Fourier transform coefficients).

- Hence, moving from periodic to non-periodic signals

  - Let $T \rightarrow \infty$,

  - Moves from the Fourier series to the Fourier transform,

  - Moves from discrete frequencies to continuous frequencies,

  - Moves from sums to integrals.

# From sine/cosine to complex exponentials

## Fourier series intuition

- $f(t) = \frac{a_{0}}{2} + \sum_{n = 1}^{\infty}\left\lbrack a_{n}cos(2\pi n\xi t) + b_{n}sin(2\pi n\xi t) \right\rbrack$ (1)

## Euler's formula

- $e^{ix} = cos(x) + i\ sin(x)$

<!-- -->

- Thus,

  - $cos(x) = \frac{e^{ix} + \ e^{- ix}}{2}$

  - $sin(x) = \frac{e^{ix} - \ e^{- ix}}{2i}$

## Plug into **Fourier series intuition**

- $f(t) = \frac{a_{0}}{2} + \sum_{n = 1}^{\infty}\left\lbrack a_{n}cos(2\pi n\xi t) + b_{n}sin(2\pi n\xi t) \right\rbrack$ (1)

> $f(t) = \frac{a_{0}}{2} + \sum_{n = 1}^{\infty}\left\lbrack a_{n}\frac{e^{i2\pi n\xi} + \ e^{- i2\pi n\xi}}{2} + b_{n}\frac{e^{i2\pi n\xi} - \ e^{- i2\pi n\xi}}{2i} \right\rbrack$
>
> $f(t) = \frac{a_{0}}{2} + \sum_{n = 1}^{\infty}\left\lbrack (\frac{a_{n}}{2} + \frac{b_{n}}{2i})e^{i2\pi n\xi} + (\frac{a_{n}}{2} - \frac{b_{n}}{2i})e^{- i2\pi n\xi} \right\rbrack$

$f(t) = \sum_{n = - \infty}^{\infty}c_{n}e^{i2\pi n\xi t}$ (2)

- For

$c_{n} = (\frac{a_{n}}{2} + \frac{b_{n}}{2i})$ for $n > 0$

$c_{- n} = (\frac{a_{n}}{2} - \frac{b_{n}}{2i})$ for $n > 0$

$c_{0} = \frac{a_{0}}{2}$

## Conclusion

- $f(t) = \frac{a_{0}}{2} + \sum_{n = 1}^{\infty}\left\lbrack a_{n}cos(2\pi n\xi t) + b_{n}sin(2\pi n\xi t) \right\rbrack$ (1)

> is simplified to

$f(t) = \sum_{n = - \infty}^{\infty}c_{n}e^{i2\pi n\xi t}$ (2)

- Complex exponentials appear.

- Positive and negative frequencies appear.

# From Fourier series intuition to Fourier series coefficients

- $f(t) = \sum_{n = - \infty}^{\infty}c_{n}e^{i2\pi n\xi t}$ (2)

- Multiply by $e^{- i2\pi m\xi t}$ and take the integral on both sides

> $\int_{0}^{T}f(t)\ e^{- i2\pi m\xi t}dt = \int_{0}^{T}\sum_{n = - \infty}^{\infty}c_{n}e^{i2\pi(n - m)\xi t}dt$
>
> $\int_{0}^{T}f(t)\ e^{- i2\pi m\xi t}dt = \sum_{n = - \infty}^{\infty}c_{n}\int_{0}^{T}e^{i2\pi(n - m)\xi t}dt$

- Observe that $\int_{0}^{T}e^{i2\pi(n - m)\xi t}dt = T$ for $n \neq m$ else $0$ (orthogonality of the $e^{i2\pi k\xi t}$ functions)

  - If $n \neq m$

> $\int_{0}^{T}e^{i2\pi(n - m)\xi t}dt$
>
> $= \left\lbrack \frac{1}{i2\pi(n - m)\xi}e^{i2\pi(n - m)\xi t} \right\rbrack_{0}^{T}$
>
> $= \frac{1}{i2\pi(n - m)\xi}(e^{i2\pi(n - m)\xi T} - 1)$
>
> $= \frac{1}{i2\pi(n - m)\xi}(e^{i2\pi(n - m)} - 1)$ because $\xi = \frac{1}{T}$
>
> $= \frac{1}{i2\pi(n - m)\xi}(1 - 1)$
>
> $= 0$

- if $n = m$

> $\int_{0}^{T}e^{i2\pi(n - m)\xi t}dt$
>
> $= \int_{0}^{T}1\ dt$
>
> $= T$

- Thus,

> $\int_{0}^{T}f(t)\ e^{- i2\pi m\xi t}dt = \sum_{n = - \infty}^{\infty}c_{n}\int_{0}^{T}e^{i2\pi(n - m)\xi t}dt = c_{m}\ T$
>
> $c_{m} = \frac{1}{T}\int_{0}^{T}f(t)\ e^{- i2\pi m\xi t}dt$

# From Fourier decomposition to Fourier transform coefficients

- $f(t) = \int_{- \infty}^{\infty}F(\xi)e^{i2\pi\xi t}d\xi$ (3)

- Multiply by $e^{- i2\pi\nu t}$ and take the integral on both sides

> $\int_{- \infty}^{\infty}f(t)\ e^{- i2\pi\nu t}dt = \int_{- \infty}^{\infty}\left( \int_{- \infty}^{\infty}F(\xi)e^{i2\pi\xi t}d\xi \right)e^{- i2\pi\nu t}dt$
>
> $\int_{- \infty}^{\infty}f(t)\ e^{- i2\pi\nu t}dt = \int_{- \infty}^{\infty}F(\xi)\left( \int_{- \infty}^{\infty}e^{i2\pi(\xi - \nu)t}dt \right)d\xi$

- Observe that $\int_{- \infty}^{\infty}e^{i2\pi(\xi - \nu)t}dt = \delta(\xi - \nu)$ (orthogonality of the $e^{i2\pi\xi t}$ functions)

- Thus,

> $\int_{- \infty}^{\infty}f(t)\ e^{- i2\pi\nu t}dt = \int_{- \infty}^{\infty}F(\xi)\left( \int_{- \infty}^{\infty}e^{i2\pi(\xi - \nu)t}dt \right)d\xi = F(\nu)$
>
> $F(\nu) = \int_{- \infty}^{\infty}f(t)\ e^{- i2\pi\nu t}dt$

## 3. Why the Fourier Transform Works

### 3.3 Convergence and real signals

- High-level convergence conditions (Dirichlet)

- Almost always satisfied by real audio

- Energy convergence vs pointwise convergence

## 4. Gibbs Phenomenon (limitations, not failure)

- Overshoot near discontinuities

- Consequence of LÂ² convergence

- Practical implications:

  - ringing

  - windowing

  - smoothing in spectrograms

# Sources

- [https://proofwiki.org/wiki/Definition:Fourier_Series/Historical_Note](https://proofwiki.org/wiki/Definition:Fourier_Series/Historical_Note)
